some cringe

avltree/AvlBase.lean
@@ -1,3 +1,19 @@
 import avltree.TreeBase
 
 open TreeBase_n
+
+namespace AvlBase_n
+
+/--
+An AVL Tree is a balanced binary tree where each
+node maintains a balance factor.
+
+-/
+inductive AvlTree where
+  | nil : AvlTree
+  | node : AvlTree → Int → AvlTree → AvlTree
+deriving Repr
+-- node(left_subtree, balance_factor, right_subtree)
+
+
+end AvlBase_n
