avltree/InductionDemo.lean
@@ -1,0 +1,36 @@
+namespace InductionDemo_n
+
+def Nat.geom_sum_powers_two : Nat → Nat
+  | 0 => 1
+  | n + 1 => Nat.geom_sum_powers_two n + Nat.pow 2 (n + 1)
+
+-- 1 + 2 + 4 + ... + 2^n = 2^(n+1) - 1
+theorem sum_geom_series : ∀ n : Nat , Nat.geom_sum_powers_two n = Nat.pow 2 (n + 1) - 1 := by
+  intro n
+  induction n with
+  | zero =>
+    simp [Nat.geom_sum_powers_two]
+  | succ n ih =>
+    simp [Nat.geom_sum_powers_two, ih]
+    grind
+
+def Nat.factorial : Nat → Nat
+  | 0 => 1
+  | n + 1 => (n + 1) * Nat.factorial n
+
+-- for all n, n! ≥ 1
+theorem factorial_ge_1 : ∀ n : Nat, Nat.factorial n ≥ 1 := by
+  intro n
+  induction n with
+  | zero =>
+    simp [Nat.factorial]
+  | succ n ih =>
+    rw [Nat.factorial]
+
+    have h1 : Nat.factorial n ≥ 1 := ih
+    have h2 : (n + 1) ≥ 1 := by
+      apply Nat.succ_le_succ
+      exact Nat.zero_le n
+    exact Nat.mul_le_mul h2 h1
+
+end InductionDemo_n
