avltree/TreeBalance.lean
@@ -1,0 +1,54 @@
+import avltree.TreeBase
+
+open TreeBase_n
+
+namespace TreeBalance_n
+
+/--
+Compute the balance factor of a binary tree.
+-/
+@[simp]
+def balanceFactor : BinaryTree → Int
+  | BinaryTree.nil => 0
+  | BinaryTree.node left right => Int.ofNat (height left) - Int.ofNat (height right)
+
+
+/--
+AVL balance condition.
+-/
+@[simp]
+def isAVL : BinaryTree → Bool
+  | BinaryTree.nil => true
+  | BinaryTree.node left right =>
+    let bf := balanceFactor (BinaryTree.node left right)
+    bf ≥ -1 ∧ bf ≤ 1 ∧ isAVL left ∧ isAVL right
+
+
+/--
+For any binary tree T, max(size T) = 2^(height T) - 1.
+-/
+theorem max_size_eq : ∀ tree : BinaryTree, size tree < 2 ^ (height tree + 1) := by
+  sorry
+
+
+/--
+We state that h(AvlTree) = O(log(size(AvlTree))).
+I.e., ∃ C, ∀ t : AvlTree, height t ≤ C * log(size t).
+I.e., size t ≥ C ^ (height t).
+-/
+theorem height_size_pow_bound :
+  ∃ C : Nat, ∀ t : BinaryTree, isAVL t → Nat.pow C (height t) ≤ size t := by
+  sorry
+
+
+
+
+
+
+
+
+
+
+
+
+end TreeBalance_n
